Progress on Test in backend

compiler/backend/data_to_wordScript.sml
@@ -1611,6 +1611,21 @@ val def = assign_Define `
       : 'a wordLang$prog # num`;
 
 val def = assign_Define `
+  assign_BoolTest (l:num) (dest:num) (test: ast$test) v1 v2 =
+                 (If Equal (adjust_var v1) (Reg (adjust_var v2))
+                   (Assign (adjust_var dest) TRUE_CONST)
+                   (Assign (adjust_var dest) FALSE_CONST),l)
+      : 'a wordLang$prog # num`;
+
+val def = assign_Define `
+  assign_WordTest (l:num) (dest:num) (test: ast$test) v1 v2 =
+                 (If (dtcase test of Equal => Equal | _ => Lower)
+                   (adjust_var v1) (Reg (adjust_var v2))
+                   (Assign (adjust_var dest) TRUE_CONST)
+                   (Assign (adjust_var dest) FALSE_CONST),l)
+      : 'a wordLang$prog # num`;
+
+val def = assign_Define `
   assign_BoundsCheckByte (c:data_to_word$config) (secn:num)
              (l:num) (dest:num) (names:num_set option) leq v1 v2 =
                    (list_Seq [Assign 1
@@ -2380,6 +2395,8 @@ Definition assign_def:
     | Label n => (LocValue (adjust_var dest) n,l)
     | MemOp (CopyByte alloc_new) => assign_CopyByte c secn l dest names args
     | MemOp RefArray => arg2 args (assign_RefArray c secn l dest names) (Skip,l)
+    | BlockOp (BoolTest test) => arg2 args (assign_BoolTest l dest test) (Skip,l)
+    | WordOp (WordTest ws test) => arg2 args (assign_WordTest l dest test) (Skip,l)
     | BlockOp (FromList tag) => arg2 args (assign_FromList c secn l dest names tag) (Skip,l)
     | IntOp (LessConstSmall i) => arg1 args (assign_LessConstSmall l dest i) (Skip,l)
     | MemOp (BoundsCheckByte leq) =>
